C# test passes

Source/DafnyStandardLibraries/src/DafnyStdLibs/MutableCollections/CSharp/Dictionary.cs
@@ -1,0 +1,18 @@
+using System.Collections.Generic;
+using System.Numerics;
+
+namespace System.Collections.Generic {
+  partial class __default {
+    public static BigInteger DictionaryLength<K,V>(IDictionary<K,V> dic) {
+      return dic.Count;
+    }
+
+    public static void DictionarySet<K,V>(IDictionary<K,V> dic, K k, V v) {
+      dic[k] = v;
+    }
+
+    public static V DictionaryGet<K,V>(IDictionary<K,V> dic, K k) {
+      return dic[k];
+    }
+  }
+}
