Source/DafnyStandardLibraries/src/DafnyStdLibs/MutableCollections/MutableCollections.dfy
@@ -3,39 +3,18 @@ include "/Users/rwillems/SourceCode/dafny2/Source/DafnyStandardLibraries/src/Daf
 module DafnyStdLibs.MutableCollections {
   import opened Wrappers
   
-  class {:extern} MutableMap<K(==),V(==)> extends MutableIteratorSource {
+  class {:extern} MutableMap<K(==),V(==)> {
      
     constructor {:extern} ()
       ensures this.content() == map[]
-      ensures version() == 0
   
-    ghost function {:extern} version(): nat reads this
     ghost function {:extern} content(): map<K, V> reads this
   
     method {:extern} Put(k: K, v: V)
       modifies this
-      ensures this.version() == old(this.version()) + 1 
       ensures this.content() == old(this.content())[k := v]
       ensures k in old(this.content()).Keys ==> this.content().Values + {old(this.content())[k]} == old(this.content()).Values + {v}
       ensures k !in old(this.content()).Keys ==> this.content().Values == old(this.content()).Values + {v}
-    
-    function {:extern} Keys(): (keys: MutableIterator<K>)
-      reads this
-      ensures keys.version() == version()
-      ensures keys.remainingElements() == content().Keys
-      ensures keys.source() == this
-  
-    function {:extern} Values(): (values: MutableIterator<V>)
-      reads this
-      ensures values.version() == version()
-      ensures values.remainingElements() == content().Values
-      ensures values.source() == this
-  
-    function {:extern} Items(): (items: MutableIterator<(K,V)>)
-      reads this
-      ensures items.version() == version()
-      ensures items.remainingElements() == set k | k in this.content().Keys :: (k, this.content()[k])
-      ensures items.source() == this
   
     predicate {:extern} HasKey(k: K)
       reads this
@@ -66,36 +45,5 @@ module DafnyStdLibs.MutableCollections {
     function {:extern} Size(): (size: int)
       reads this
       ensures size == |this.content().Items|
-  }
-  
-  
-  trait {:termination false} MutableIterator<T(==)> {
-    ghost function version(): nat reads this
-    ghost function source(): MutableIteratorSource reads this
-    ghost function remainingElements(): set<T> reads this
-    var wasInterrupted: bool
-    ghost function current(): Option<T> reads this
-    
-    function {:extern} WasInterrupted(): (r: bool) {
-      wasInterrupted
-    }
-    
-    method {:extern} MoveNext() returns (r: bool)
-      modifies this
-      ensures (version() != source().version()) == wasInterrupted
-      ensures current().Some? == r
-      ensures if (!wasInterrupted && |remainingElements()| > 0) 
-        then r && var value := current().Extract(); { value } + remainingElements() == old(remainingElements()) 
-               && 1 + |remainingElements()| == |old(remainingElements())|
-        else !r && old(remainingElements) == remainingElements
-
-    function {:extern} Current(): (v: T)
-      reads this
-      requires current().Some?
-      ensures v == current().Extract()
-  }
-  
-  trait {:termination false} MutableIteratorSource {
-    ghost function version(): nat reads this
   }
 }
