Source/DafnyStandardLibraries/examples/MutableCollectionsExamples.dfy
@@ -1,53 +1,66 @@
+include "/Users/rwillems/SourceCode/dafny2/Source/DafnyStandardLibraries/src/DafnyStdLibs/MutableCollections/CSharp/Dictionary.cs.dfy"
+include "/Users/rwillems/SourceCode/dafny2/Source/DafnyStandardLibraries/src/DafnyStdLibs/MutableCollections/CSharp/MutableCollection.cs.dfy"
 
-include "/Users/rwillems/SourceCode/dafny2/Source/DafnyStandardLibraries/src/DafnyStdLibs/MutableCollections/MutableCollections.dfy"
+// include "/Users/rwillems/SourceCode/dafny2/Source/DafnyStandardLibraries/src/DafnyStdLibs/MutableCollections/MutableCollections.dfy"
 
 module Example {
   import opened DafnyStdLibs.MutableCollections
 
-  method {:test} TraverseKeysWithoutInterruption() {
+  method {:test} PutGet() {
     var m := new MutableMap<int, int>();
     m.Put(3, 2);
     m.Put(4, 1);
-    
-    var s: set<int> := {};
-    var keyIterator := m.Keys();
-    var hasNext := keyIterator.MoveNext();
-    while(hasNext)
-      decreases hasNext, |keyIterator.remainingElements|
-      invariant !keyIterator.WasInterrupted()
-      invariant keyIterator.current.Some? ==> { keyIterator.current.Extract() } + s + keyIterator.remainingElements == m.content().Keys
-      invariant keyIterator.current.None? ==> s + keyIterator.remainingElements == m.content().Keys
-      invariant keyIterator.current.None? ==> keyIterator.remainingElements == {}
-        
-      // Surprised I need this. I thought Dafny would figure that this would does not need a modified clause
-      invariant {3,4} == m.content().Keys
-    {
-      var currentKey := keyIterator.Current();
-      s := s + {currentKey};
-      hasNext := keyIterator.MoveNext();
-    }
-        
-    assert s == {3, 4};
+
+    var x := m.Select(3);
+    var y := m.Select(4);
+    expect x == 2;
+    expect y == 1;
   }
 
-  method {:test} TraverseKeysWithInterruption() {
-    var m := new MutableMap<int, int>();
-    m.Put(3, 2);
-    m.Put(4, 1);
+  // method {:test} TraverseKeysWithoutInterruption() {
+  //   var m := new MutableMap<int, int>();
+  //   m.Put(3, 2);
+  //   m.Put(4, 1);
     
-    var s: set<int> := {};
-    var keyIterator := m.Keys();
-    m.Put(5, 0);
-    var hasNext := keyIterator.MoveNext();
-    while(hasNext)
-      decreases hasNext, |keyIterator.remainingElements|
-      invariant s == {}
-    {
-      var currentKey := keyIterator.Current();
-      s := s + {currentKey};
-      hasNext := keyIterator.MoveNext();
-    }
+  //   var s: set<int> := {};
+  //   var keyIterator := m.Keys();
+  //   var hasNext := keyIterator.MoveNext();
+  //   while(hasNext)
+  //     decreases hasNext, |keyIterator.remainingElements|
+  //     invariant !keyIterator.WasInterrupted()
+  //     invariant keyIterator.current.Some? ==> { keyIterator.current.Extract() } + s + keyIterator.remainingElements == m.content().Keys
+  //     invariant keyIterator.current.None? ==> s + keyIterator.remainingElements == m.content().Keys
+  //     invariant keyIterator.current.None? ==> keyIterator.remainingElements == {}
+        
+  //     // Surprised I need this. I thought Dafny would figure that this would does not need a modified clause
+  //     invariant {3,4} == m.content().Keys
+  //   {
+  //     var currentKey := keyIterator.Current();
+  //     s := s + {currentKey};
+  //     hasNext := keyIterator.MoveNext();
+  //   }
+        
+  //   assert s == {3, 4};
+  // }
+
+  // method {:test} TraverseKeysWithInterruption() {
+  //   var m := new MutableMap<int, int>();
+  //   m.Put(3, 2);
+  //   m.Put(4, 1);
     
-    assert s == {};
-  }
+  //   var s: set<int> := {};
+  //   var keyIterator := m.Keys();
+  //   m.Put(5, 0);
+  //   var hasNext := keyIterator.MoveNext();
+  //   while(hasNext)
+  //     decreases hasNext, |keyIterator.remainingElements|
+  //     invariant s == {}
+  //   {
+  //     var currentKey := keyIterator.Current();
+  //     s := s + {currentKey};
+  //     hasNext := keyIterator.MoveNext();
+  //   }
+    
+  //   assert s == {};
+  // }
 }
